Give more structure to capture groups

RegexCorrectness/Data/Expr/Semantics/Captures.lean
@@ -1,36 +1,38 @@
 import Regex.Data.Expr
 import RegexCorrectness.Data.Span
+import RegexCorrectness.Data.Expr.Semantics.CaptureGroups
 import RegexCorrectness.Data.Expr.Semantics.Matches
 
 set_option autoImplicit false
 
 namespace Regex.Data
 
-inductive Expr.Captures : Span → Span → List (Nat × String.Pos × String.Pos) → Expr → Prop where
-  | char {l m r} (c : Char) : Expr.Captures ⟨l, m, c :: r⟩ ⟨l, c :: m, r⟩ [] (.char c)
-  | sparse {l m c r cs} (h : c ∈ cs) : Expr.Captures ⟨l, m, c :: r⟩ ⟨l, c :: m, r⟩ [] (.classes cs)
-  | epsilon {span} : Expr.Captures span span [] .epsilon
+inductive Expr.Captures : Span → Span → CaptureGroups → Expr → Prop where
+  | char {l m r} (c : Char) : Expr.Captures ⟨l, m, c :: r⟩ ⟨l, c :: m, r⟩ .empty (.char c)
+  | sparse {l m c r cs} (h : c ∈ cs) : Expr.Captures ⟨l, m, c :: r⟩ ⟨l, c :: m, r⟩ .empty (.classes cs)
+  | epsilon {span} : Expr.Captures span span .empty .epsilon
   | group {span span' groups tag e} (cap : Expr.Captures span span' groups e) :
-    Expr.Captures span span' (groups ++ [(tag, span.curr, span'.curr)]) (.group tag e)
+    Expr.Captures span span' (.group tag span.curr span'.curr groups) (.group tag e)
   | alternateLeft {span span' groups e₁ e₂} (cap : Expr.Captures span span' groups e₁) :
     Expr.Captures span span' groups (.alternate e₁ e₂)
   | alternateRight {span span' groups e₁ e₂} (cap : Expr.Captures span span' groups e₂) :
     Expr.Captures span span' groups (.alternate e₁ e₂)
   | concat {span span' span'' groups₁ groups₂ e₁ e₂} (cap₁ : Expr.Captures span span' groups₁ e₁) (cap₂ : Expr.Captures span' span'' groups₂ e₂) :
-    Expr.Captures span span'' (groups₁ ++ groups₂) (.concat e₁ e₂)
-  | starEpsilon {span e} : Expr.Captures span span [] (.star e)
-  | starConcat {span span' span'' groups groups' e} (cap₁ : Expr.Captures span span' groups e) (cap₂ : Expr.Captures span' span'' groups' (.star e)) :
-    Expr.Captures span span'' (groups ++ groups') (.star e)
+    Expr.Captures span span'' (.concat groups₁ groups₂) (.concat e₁ e₂)
+  | starEpsilon {span e} : Expr.Captures span span .empty (.star e)
+  | starConcat {span span' span'' groups₁ groups₂ e} (cap₁ : Expr.Captures span span' groups₁ e) (cap₂ : Expr.Captures span' span'' groups₂ (.star e)) :
+    Expr.Captures span span'' (.concat groups₁ groups₂) (.star e)
 
+-- NOTE: this will not be true once we add anchors (^ and $).
 theorem captures_of_matches {l n₁ n₂ r e} (m : Expr.matches n₂ e) :
   ∃ groups, Expr.Captures ⟨l, n₁, n₂ ++ r⟩ ⟨l, n₂.reverse ++ n₁, r⟩ groups e := by
   induction m generalizing n₁ r with
-  | char c => exact ⟨[], .char c⟩
-  | sparse cs c mem => exact ⟨[], .sparse mem⟩
-  | epsilon => exact ⟨[], .epsilon⟩
+  | char c => exact ⟨.empty, .char c⟩
+  | sparse cs c mem => exact ⟨.empty, .sparse mem⟩
+  | epsilon => exact ⟨.empty, .epsilon⟩
   | group m ih =>
     have ⟨groups, cap⟩ := @ih n₁ r
-    exact ⟨groups ++ [_], .group cap⟩
+    exact ⟨.group _ _ _ groups, .group cap⟩
   | alternateLeft m ih =>
     have ⟨groups, cap⟩ := @ih n₁ r
     exact ⟨groups, .alternateLeft cap⟩
@@ -40,12 +42,12 @@ theorem captures_of_matches {l n₁ n₂ r e} (m : Expr.matches n₂ e) :
   | concat cs₁ cs₂ _ _ m₁ m₂ ih₁ ih₂ =>
     have ⟨groups₁, cap₁⟩ := @ih₁ n₁ (cs₂ ++ r)
     have ⟨groups₂, cap₂⟩ := @ih₂ (cs₁.reverse ++ n₁) r
-    exact ⟨groups₁ ++ groups₂, by simp; exact .concat cap₁ cap₂⟩
-  | starEpsilon => exact ⟨[], .starEpsilon⟩
+    exact ⟨.concat groups₁ groups₂, by simp; exact .concat cap₁ cap₂⟩
+  | starEpsilon => exact ⟨.empty, .starEpsilon⟩
   | starConcat cs₁ cs₂ _ _ _ ih₁ ih₂ =>
     have ⟨groups₁, cap₁⟩ := @ih₁ n₁ (cs₂ ++ r)
     have ⟨groups₂, cap₂⟩ := @ih₂ (cs₁.reverse ++ n₁) r
-    exact ⟨groups₁ ++ groups₂, by simp; exact .starConcat cap₁ cap₂⟩
+    exact ⟨.concat groups₁ groups₂, by simp; exact .starConcat cap₁ cap₂⟩
 
 theorem matches_of_captures {span span' groups e} (c : Expr.Captures span span' groups e) :
   ∃ n, Expr.matches n e ∧ span'.l = span.l ∧ span'.m = n.reverse ++ span.m ∧ n ++ span'.r = span.r := by
